{
 "cells": [
  {
   "cell_type": "markdown",
   "metadata": {
    "id": "Htm5D9RhL994"
   },
   "source": [
    "### Homework Assignment #4\n",
    "\n",
    "#### Question 1: Convolution Theorem\n",
    "\n",
    "**a. Convolution in Fourier Space**: Prove that the Fourier transform of the convolution of two functions $f$ and $g$, denoted as $\\mathcal{F}(f \\star g)$, equals the pointwise product of their Fourier transforms:  \n",
    "$$\n",
    "\\mathcal{F}(f \\star g) = \\mathcal{F}(f) \\cdot \\mathcal{F}(g).\n",
    "$$  \n",
    "Specify whether your proof is for continuous functions or discrete signals and clearly state any assumptions made.\n",
    "\n",
    "---\n",
    "\n",
    "#### Question 2: Properties of Convolution\n",
    "\n",
    "**a. Commutativity**: Prove that the convolution operation is commutative:  \n",
    "$$\n",
    "f \\star g = g \\star f.\n",
    "$$\n",
    "\n",
    "**b. Distributivity**: Prove the distributive property of convolution:  \n",
    "$$\n",
    "f \\star (\\alpha g + \\beta h) = \\alpha (f \\star g) + \\beta (f \\star h),\n",
    "$$  \n",
    "where $ \\alpha, \\beta \\in \\mathbb{R} $.\n",
    "\n",
    "**c. Shift Equivariance**: Prove that convolution is shift-invariant:  \n",
    "$$\n",
    "f(x) \\star g(x - d) = (f \\star g)(x - d).\n",
    "$$\n",
    "\n",
    "**d. Scaling Property**: Prove that if a function $ f(x) $ is scaled in its argument by a factor $ a > 0 $, then its convolution with a function $ g(x) $ satisfies:  \n",
    "$$\n",
    "f(ax) \\star g(ax) = \\frac{1}{a} \\big(f \\star g\\big)(ax).\n",
    "$$\n",
    "Clearly state any assumptions and steps in your proof.\n",
    "\n",
    "---\n",
    "\n",
    "#### Question 3: Derivative and Inverse of Convolution\n",
    "\n",
    "**a. Derivative of Convolution**: Derive the expression for the derivative of the convolution $ f(x) \\star g(x) $:  \n",
    "$$\n",
    "\\frac{d}{dx} \\big(f(x) \\star g(x)\\big).\n",
    "$$  \n",
    "Verify this property for specific functions of your choice, such as $ f(x) = e^{-x^2} $ and $ g(x) = \\sin(x) $.\n",
    "\n",
    "**b. Inverse of Convolution**: Discuss the conditions under which the convolution $ f(x) \\star g(x) $ can be inverted. Derive the theoretical framework for deconvolution or solving for $ f(x) $ or $ g(x) $ given their convolution.\n",
    "\n",
    "---\n",
    "\n",
    "#### Question 4 (Optional, Coding): Practical Verification of Convolution Properties\n",
    "\n",
    "**a. Implementation**: Implement the convolution operation using Python (e.g., PyTorch or NumPy) and verify the properties discussed in Question 2 for specific example functions $ f(x) $ and $ g(x) $.  \n",
    "\n",
    "**b. Fourier Transform Connection**: Use the Fourier transform to verify the convolution theorem numerically. Show that $ \\mathcal{F}(f \\star g) = \\mathcal{F}(f) \\cdot \\mathcal{F}(g) $ for your chosen functions $ f(x) $ and $ g(x) $.\n",
    "\n",
    "**c. Applications**: Briefly explain how these properties are utilized in convolutional neural networks (CNNs)."
   ]
  },
  {
   "cell_type": "markdown",
   "metadata": {},
   "source": [
    "## Solution\n",
    "Question 1:\n",
    "$$\n",
    "\\mathcal{F}(f \\star g) = \\mathcal{F}(f) \\cdot \\mathcal{F}(g).\n",
    "$$  \n",
    "Proof:\n",
    "$$\n",
    "\\mathcal{F}(f \\star g) =\\int_{-\\infty}^{\\infty} f \\star g \\ e^{-2 \\pi i \\omega t}dt = \\int_{-\\infty}^{\\infty} (\\int_{-\\infty}^{\\infty} f(s) \\ g\n",
    "(t-s) ds) \\ e^{-2 \\pi i \\omega t}dt = \n",
    "$$\n",
    "$$\n",
    "= \\int_{-\\infty}^{\\infty} f(s) (\\int_{-\\infty}^{\\infty}  \\ g(t-s) e^{-2 \\pi i \\omega t} dt) \\ ds = \\{ \\hat{t} = t-s , d\\hat{t}=dt \\} = \\int_{-\\infty}^{\\infty} f(s) (\\int_{-\\infty}^{\\infty}  \\ g(\\hat t) e^{-2 \\pi i \\omega (\\hat t +s)} d\\hat t) \\ ds =\n",
    "$$\n",
    "$$\n",
    "= \\int_{-\\infty}^{\\infty} f(s) e^{-2 \\pi i \\omega s} (\\int_{-\\infty}^{\\infty}  \\ g(\\hat t) e^{-2 \\pi i \\omega \\hat t} d\\hat t) \\ ds =\n",
    "\\mathcal{F}(f) \\cdot \\mathcal{F}(g). \\\\\n",
    "\\text{End of proof}\n",
    "$$\n",
    "Assumptions: \\\n",
    "1) We can change the order of integration.\\\n",
    "2) We deal with continues funciton f,g for which the Fourier Transform exists.\\\n",
    "<br>\n",
    "I will add that the formula for convolution is:\n",
    "$$\n",
    "f \\star g (t) =\\int_{-\\infty}^{\\infty} f(s) \\ g(t-s) ds \n",
    "$$"
   ]
  },
  {
   "cell_type": "markdown",
   "metadata": {},
   "source": [
    "#### Question 2: Properties of Convolution\n",
    "**a. Commutativity**\n",
    "$$\n",
    "f \\star g = g \\star f.\n",
    "$$\n",
    "Proof\n",
    "$$\n",
    "f \\star g (t) = \\int_{-\\infty}^{\\infty} f(s) \\ g(t-s) ds = \\{  s = t - \\hat s, ds = -d \\hat s \\} =\n",
    "\\int_{\\infty}^{-\\infty} f(t- \\hat s) \\ g(\\hat s) - d \\hat s =\n",
    "$$\n",
    "$$\n",
    "=\\int_{-\\infty}^{\\infty} f(t- \\hat s) \\ g(\\hat s) d \\hat s \n",
    "\n",
    "=g \\star f.\n",
    "\n",
    "$$\n",
    "End of proof.\n",
    "\n",
    "**b. Distributivity**: \n",
    "$$\n",
    "f \\star (\\alpha g + \\beta h) \n",
    "= \\int_{-\\infty}^{\\infty} f(s) \\ (\\alpha g + \\beta h)(t-s) ds \n",
    "=\\int_{-\\infty}^{\\infty} f(s) \\ (\\alpha g(t-s) + \\beta h (t-s)) ds=\n",
    "$$\n",
    "$$\n",
    "= \\alpha \\int_{-\\infty}^{\\infty} f(s) \\ g(t-s) ds +\\beta \\int_{-\\infty}^{\\infty} f(s) \\ h (t-s)ds\n",
    "=\\alpha (f \\star g) + \\beta (f \\star h),\n",
    "$$  \n",
    "End of proof. \n",
    "\n",
    "Assumpotions: \n",
    "1) We work on a linear space in which: <br>\n",
    "$(\\alpha g)(t-s) = \\alpha g(t-s)$, \\\n",
    "$(g + h)(t-s) = g(t-s) +  h (t-s)$ \n",
    "2) $ \\alpha, \\beta \\in \\mathbb{R} $.\n",
    "\n",
    "\n",
    "\n",
    "**c. Shift Equivariance**:\n",
    "$$\n",
    "\\text{Let's notate: }\n",
    "$$\n",
    "$$\n",
    "h(x) = g(x-d)\n",
    "$$\n",
    "$$\n",
    "\\text{On the one hand, }\n",
    "f(x) \\star g(x - d) = f(x) \\star h(x) =\\int_{-\\infty}^{\\infty} f(s) \\ h(x-s) ds \n",
    "= \\int_{-\\infty}^{\\infty} f(s) \\ g(x-d-s) ds \n",
    "$$\n",
    "$$\n",
    "\\text{Let's notate: } \n",
    "$$\n",
    "$$\n",
    "\\hat{x}=x-d\n",
    "$$\n",
    "$$\n",
    "\\text{On the one hand, }\n",
    "(f \\star g)(x - d)= (f \\star g)(\\hat{x})=\\int_{-\\infty}^{\\infty} f(s) \\ g(\\hat{x}-s) ds = \n",
    "\\int_{-\\infty}^{\\infty} f(s) \\ g(x-d-s) ds \n",
    "$$\n",
    "$$\n",
    "\\text{Therefore, }\n",
    "$$\n",
    "$$\n",
    "f(x) \\star g(x - d) = (f \\star g)(x - d)\n",
    "$$\n",
    "End of proof.\n",
    "\n",
    "**d. Scaling Property**: \\\n",
    "$a>0$\n",
    "$$\n",
    "\\text{Let's notate: }\n",
    "$$\n",
    "$$\n",
    "\\hat f(x) = f(ax),\n",
    "$$\n",
    "$$\n",
    "\\hat g(x) = g(ax) \n",
    "$$\n",
    "$$\n",
    "f(ax) \\star g(ax) = \\hat f(x) \\star \\hat g(x) =\\int_{-\\infty}^{\\infty} \\hat f(s) \\ \\hat g(x-s) ds =\n",
    "$$\n",
    "$$\n",
    "= \\int_{-\\infty}^{\\infty} f(as) \\  g(a(x-s)) ds= | \\hat s =as , ds = \\frac{1}{a} \\ d\\hat s| = \\frac{1}{a} \\int_{-\\infty}^{\\infty} f(\\hat s) \\ g(ax- \\hat s) d\\hat s=\\frac{1}{a} \\big(f \\star g\\big)(ax).\n",
    "$$\n",
    "End of proof.\n"
   ]
  },
  {
   "cell_type": "markdown",
   "metadata": {},
   "source": [
    "\n",
    "#### Question 3\n",
    "\n",
    "**a. Derivative of Convolution**: Derive the expression for the derivative of the convolution $ f(x) \\star g(x) $:  \n",
    "$$\n",
    "\\frac{d}{dx} \\big(f(x) \\star g(x)\\big).\n",
    "$$  \n",
    "Proof:\n",
    "$$\n",
    "\\frac{d}{dx} \\big(f(x) \\star g(x)\\big) =  \\frac{d}{dx} \\int_{-\\infty}^{\\infty} f(s) \\ g(x-s) ds =\n",
    "$$\n",
    "$$\n",
    "=\\int_{-\\infty}^{\\infty} \\frac{d}{dx} f(s) \\ g(x-s) ds = \\int_{-\\infty}^{\\infty} f(s) \\ g'(x-s) ds \n",
    "= \\big(f(x) \\star g'(x)  \\big) = \\big(f \\star \\frac{dg}{dx}  \\big).\n",
    "$$\n",
    "$$\n",
    "\\text{ In the same way:}\n",
    "$$\n",
    "$$\n",
    "\\frac{d}{dx} \\big(f(x) \\star g(x)\\big) = \\frac{d}{dx} \\big(g(x) \\star f(x)\\big) \n",
    "= \\big(g \\star \\frac{df}{dx}  \\big) = \\big(\\frac{df}{dx} \\star g \\big).\n",
    "$$\n",
    "$$\n",
    "\\text{ So in conclusion, we got: }\n",
    "$$\n",
    "$$\n",
    "\\frac{d}{dx} \\big(f(x) \\star g(x)\\big) =  \\big(f(x) \\star \\frac{d g}{dx}\\big) =  \\big(\\frac{df}{dx} \\star g(x)\\big)\n",
    "$$\n",
    "Let's verify this property for specific functions:\n",
    "$$\n",
    "g(x) = x^2\n",
    "$$\n",
    "$$\n",
    "g'(x)=2x\n",
    "$$\n",
    "$$\n",
    "f(x)=\n",
    "\\begin{cases} \n",
    "x, & -1 \\leq x < 0, \\\\\n",
    "-x, & 0 \\leq x \\leq 1, \\\\\n",
    "0, & \\text{otherwise}.\n",
    "\\end{cases}\n",
    "$$\n",
    "$$\n",
    "\\frac{d}{dx}(f(x) \\star g(x)) = \\frac{d}{dx} \\int_{-\\infty}^{\\infty}f(s) \\ g(x-s) ds =\n",
    "$$\n",
    "$$\n",
    "= \\frac{d}{dx} (\\int_{-1}^{0} s \\ (x-s)^2 ds + \\int_{0}^{1} -s \\ (x-s)^2 ds)=\n",
    "$$\n",
    "$$\n",
    "= \\frac{d}{dx} (\\int_{-1}^{0} s \\ (x^2-2xs+s^2) ds - \\int_{0}^{1} s \\ (x^2-2xs+s^2) ds)\n",
    "$$\n",
    "$$\n",
    "= \\frac{d}{dx} (\\int_{-1}^{0} (x^2 s-2xs^2+s^3) ds - \\int_{0}^{1} (x^2s-2xs^2+s^3) ds)\n",
    "$$\n",
    "$$\n",
    "=\\frac{d}{dx} (x^2 \\frac{s^2}{2}-2x\\frac{s^3}{3}+\\frac{s^4}{4}\\Big|_{-1}^0 - x^2 \\frac{s^2}{2}+2x\\frac{s^3}{3}-\\frac{s^4}{4}\\Big|_{0}^1)\n",
    "$$\n",
    "$$\n",
    "=\\frac{d}{dx}(-x^2-\\frac{1}{2})=-2x\n",
    "$$\n",
    "So,\n",
    "$$\n",
    "\\frac{d}{dx}(f(x) \\star g(x)) =-2x\n",
    "$$\n",
    "Let's check the property,\n",
    "$$\n",
    "(f(x) \\star \\frac{d}{dx}g(x)) = \\int_{-\\infty}^{\\infty}f(s) \\ g'(x-s) ds =\n",
    "$$\n",
    "$$\n",
    "= (\\int_{-1}^{0} s \\ 2(x-s) ds + \\int_{0}^{1} -s \\ 2(x-s) ds)=\n",
    "$$\n",
    "$$\n",
    "=(\\int_{-1}^{0} (2xs-2s^2) ds - \\int_{0}^{1} (2xs-2s^2) ds)= \n",
    "$$\n",
    "$$\n",
    "=xs^2-\\frac{2s^3}{3}\\Big|_{-1}^0 - xs^2+\\frac{2s^3}{3} \\Big|_{0}^1 =-2x\n",
    "$$\n",
    "So we indded see that:\n",
    "$$\n",
    "\\frac{d}{dx}(f(x) \\star g(x)) = f(x) \\star \\frac{d}{dx}g(x)\n",
    "$$\n",
    "\n",
    "#### Remark\n",
    "The function $f(x)$ isn't differentiable ( at 0, -1 and 1) so we won't check the property for it.\n",
    "<br>\n",
    "<br>\n",
    "<br>\n",
    "\n",
    "**b. Inverse of Convolution**: Discuss the conditions under which the convolution $ f(x) \\star g(x) $ can be inverted. Derive the theoretical framework for deconvolution or solving for $ f(x) $ or $ g(x) $ given their convolution.\n",
    "\n",
    "To solve that, we will need to use fourier transform, therefore we assume that there it is a fourier transform for f(x), g(x) and its convolution.\n",
    "Let's solve for $f(t)$. \n",
    "Let's notate: \n",
    "$$\n",
    "h(t) = f(t) \\star g(t)\n",
    "$$\n",
    "Let's apply fourier transform.\n",
    "$$\n",
    "\\mathcal{F}(f(t) \\star g(t)) = \\mathcal{F} (h(t))\n",
    "$$\n",
    "Let us use the convolution property of Fourier transform.\n",
    "$$\n",
    "\\mathcal{F}(f(t)) \\mathcal{F}(g(t)) = \\mathcal{F}(h(t))\n",
    "$$\n",
    "Therefore, assuming $\\mathcal{F}(g(t)) \\neq 0$\n",
    "$$\n",
    "\\mathcal{F}(f(t)) = \\frac{\\mathcal{F}(h(t))}{\\mathcal{F}(g(t))}\n",
    "$$\n",
    "We will apply inverse fourier transform.\n",
    "$$\n",
    "\\mathcal{F^{-1}}(\\mathcal{F}(f(t))) = \\mathcal{F^{-1}}(\\frac{\\mathcal{F}(h(t))}{\\mathcal{F}(g(t))})\n",
    "$$\n",
    "And we get,\n",
    "$$\n",
    "f(t) = \\mathcal{F^{-1}}(\\frac{\\mathcal{F}(h(t))}{\\mathcal{F}(g(t))})\n",
    "$$\n",
    "In the same way\n",
    "$$\n",
    "g(t) = \\mathcal{F^{-1}}(\\frac{\\mathcal{F}(h(t))}{\\mathcal{F}(f(t))})\n",
    "$$\n",
    "\n",
    "So we got:\n",
    "$$\n",
    "f(t) = \\mathcal{F^{-1}}(\\frac{\\mathcal{F}(h(t))}{\\mathcal{F}(g(t))})\n",
    "$$\n",
    "$$\n",
    "g(t) = \\mathcal{F^{-1}}(\\frac{\\mathcal{F}(h(t))}{\\mathcal{F}(f(t))})\n",
    "$$\n",
    "End."
   ]
  }
 ],
 "metadata": {
  "colab": {
   "provenance": []
  },
  "kernelspec": {
   "display_name": "Python 3",
   "name": "python3"
  },
  "language_info": {
   "name": "python"
  }
 },
 "nbformat": 4,
 "nbformat_minor": 0
}
